rustfrontend/Rusttypes.v
@@ -1,0 +1,134 @@
+(** Type for Rustlight languages  *)
+
+Require Import Axioms Coqlib Maps Errors.
+Require Import AST Linking.
+Require Import Ctypes.
+Require Archi.
+
+Set Asymmetric Patterns.
+
+Local Open Scope error_monad_scope.
+
+Inductive usekind : Type :=
+| Copy
+| Move.                        (**r used for types that are unsafe for copying *)
+
+
+(** ** Types  *)
+
+Inductive type : Type :=
+| Tunit: type                                    (**r the [unit] type *)
+| Tint: intsize -> signedness -> attr -> type       (**r integer types *)
+| Tfunction: typelist -> type -> calling_convention -> type    (**r function types *)
+| Tstruct: ident -> attr -> type                              (**r struct types  *)
+| Tunion: ident -> attr -> type                               (**r union types *)
+with typelist : Type :=
+| Tnil: typelist
+| Tcons: type -> typelist -> typelist.
+
+
+Lemma type_eq: forall (ty1 ty2: type), {ty1=ty2} + {ty1<>ty2}
+with typelist_eq: forall (tyl1 tyl2: typelist), {tyl1=tyl2} + {tyl1<>tyl2}.
+Proof.
+  assert (forall (x y: floatsize), {x=y} + {x<>y}) by decide equality.
+  generalize ident_eq zeq bool_dec ident_eq intsize_eq signedness_eq attr_eq; intros.
+  decide equality.
+  decide equality.
+  decide equality.
+  decide equality.
+Defined.
+
+(** Composite  *)
+
+Inductive member : Type :=
+  | Member_plain (id: ident) (t: type).
+
+Definition members : Type := list member.
+
+Inductive composite_definition : Type :=
+  Composite (id: ident) (su: struct_or_union) (m: members) (a: attr).
+
+Definition name_member (m: member) : ident :=
+  match m with
+  | Member_plain id _ => id
+  end.
+
+Definition type_member (m: member) : type :=
+  match m with
+  | Member_plain _ t => t
+  end.
+
+Definition member_is_padding (m: member) : bool :=
+  match m with
+  | Member_plain _ _ => false
+  end.
+
+Definition name_composite_def (c: composite_definition) : ident :=
+  match c with Composite id su m a => id end.
+
+Definition composite_def_eq (x y: composite_definition): {x=y} + {x<>y}.
+Proof.
+  decide equality.
+- decide equality. decide equality. apply N.eq_dec. apply bool_dec.
+- apply list_eq_dec. decide equality.
+  apply type_eq. apply ident_eq.
+- decide equality.
+- apply ident_eq.
+Defined.
+
+Global Opaque composite_def_eq. 
+
+(** For type-checking, compilation and semantics purposes, the composite
+  definitions are collected in the following [composite_env] environment.
+  The [composite] record contains additional information compared with
+  the [composite_definition], such as size and alignment information. *)
+
+Record composite : Type := {
+  co_su: struct_or_union;
+  co_members: members;
+  co_attr: attr;
+  co_sizeof: Z;
+  co_alignof: Z;
+  co_rank: nat;
+  co_sizeof_pos: co_sizeof >= 0;
+  co_alignof_two_p: exists n, co_alignof = two_power_nat n;
+  co_sizeof_alignof: (co_alignof | co_sizeof)
+}.
+
+Definition composite_env : Type := PTree.t composite.
+
+(** Access modes for members of structs or unions: either a plain field
+    or a bitfield *)
+
+Inductive bitfield : Type :=
+  | Full
+  | Bits (sz: intsize) (sg: signedness) (pos: Z) (width: Z).
+
+
+Section PROGRAMS.
+
+(** move to Rusttypes *)
+Variable F: Type.
+
+Inductive fundef : Type :=
+| Internal: F -> fundef
+| External: external_function -> typelist -> type -> calling_convention -> fundef.
+
+
+Record program : Type := {
+  prog_defs: list (ident * globdef fundef type);
+  prog_public: list ident;
+  prog_main: ident;
+  prog_types: list composite_definition;
+  prog_comp_env: composite_env;
+  prog_comp_env_eq: build_composite_env prog_types = OK prog_comp_env
+}.
+
+Definition program_of_program (p: program) : AST.program fundef type :=
+  {| AST.prog_defs := p.(prog_defs);
+     AST.prog_public := p.(prog_public);
+     AST.prog_main := p.(prog_main) |}.
+
+Coercion program_of_program: program >-> AST.program.
+
+End PROGRAMS.
